Uppaal_Networks/UPPAAL_Asm_AbsInt_Flat.thy
@@ -187,23 +187,23 @@ proof (intro Set.equalityI)
   qed
 qed
 
-definition collect_step_flat :: "program \<Rightarrow> state set \<Rightarrow> state set" where
-  "collect_step_flat prog instates = instates \<union> step_all_flat prog instates"
+definition advance_flat :: "program \<Rightarrow> state set \<Rightarrow> state set" where
+  "advance_flat prog instates = instates \<union> step_all_flat prog instates"
 
-inductive_set collect_step_flat_induct for prog instates where
-  keep: "st \<in> instates \<Longrightarrow> st \<in> collect_step_flat_induct prog instates" |
-  step: "st \<in> step_all_flat prog instates \<Longrightarrow> st \<in> collect_step_flat_induct prog instates"
+inductive_set advance_flat_induct for prog instates where
+  keep: "st \<in> instates \<Longrightarrow> st \<in> advance_flat_induct prog instates" |
+  step: "st \<in> step_all_flat prog instates \<Longrightarrow> st \<in> advance_flat_induct prog instates"
 
-lemma collect_step_flat_eq: "collect_step_flat prog instates = collect_step_flat_induct prog instates"
+lemma advance_flat_eq: "advance_flat prog instates = advance_flat_induct prog instates"
 proof
-  show "collect_step_flat prog instates \<subseteq> collect_step_flat_induct prog instates"
-    using collect_step_flat_def collect_step_flat_induct.intros(1) collect_step_flat_induct.intros(2) step_all_flat_def step_all_flat.intros by auto
-  show "collect_step_flat_induct prog instates \<subseteq> collect_step_flat prog instates"
-    using collect_step_flat_def collect_step_flat_induct.simps step_all_flat.simps by fastforce
+  show "advance_flat prog instates \<subseteq> advance_flat_induct prog instates"
+    using advance_flat_def advance_flat_induct.intros(1) advance_flat_induct.intros(2) step_all_flat_def step_all_flat.intros by auto
+  show "advance_flat_induct prog instates \<subseteq> advance_flat prog instates"
+    using advance_flat_def advance_flat_induct.simps step_all_flat.simps by fastforce
 qed
 
-lemma collect_step_flat_steps_exact:
-  assumes "outs \<in> collect_step_flat_induct prog instates"
+lemma advance_flat_steps_exact:
+  assumes "outs \<in> advance_flat_induct prog instates"
   shows "\<exists>ins\<in>instates. steps_upto prog 1 ins outs"
 using assms proof(cases)
   case keep
@@ -221,12 +221,12 @@ next
   qed
 qed
 
-lemma step_in_collect_flat: "step_all_flat prog sts \<subseteq> collect_step_flat prog sts"
-  by (simp add: collect_step_flat_def)
+lemma step_in_collect_flat: "step_all_flat prog sts \<subseteq> advance_flat prog sts"
+  by (simp add: advance_flat_def)
 
 fun collect_loop_flat :: "program \<Rightarrow> fuel \<Rightarrow> state set \<Rightarrow> state set" where
   "collect_loop_flat _ 0 instates = instates" |
-  "collect_loop_flat prog (Suc n) instates = collect_loop_flat prog n (collect_step_flat prog instates)"
+  "collect_loop_flat prog (Suc n) instates = collect_loop_flat prog n (advance_flat prog instates)"
 
 lemma collect_loop_flat_correct:
   "collect_loop_flat prog n instates = {st. \<exists>ins\<in>instates. steps_upto prog n ins st}"
@@ -240,9 +240,9 @@ proof(intro Set.equalityI Set.subsetI)
     from this nostep show ?case by blast
   next
     case (Suc fuel)
-    hence "\<exists>ins'\<in>(collect_step_flat prog instates). steps_upto prog fuel ins' x" by simp
-    from this obtain "ins'" where ins': "ins' \<in> collect_step_flat prog instates" "steps_upto prog fuel ins' x" by blast
-    from this(1) have "\<exists>ins\<in>instates. steps_upto prog 1 ins ins'" using collect_step_flat_steps_exact collect_step_flat_eq by auto
+    hence "\<exists>ins'\<in>(advance_flat prog instates). steps_upto prog fuel ins' x" by simp
+    from this obtain "ins'" where ins': "ins' \<in> advance_flat prog instates" "steps_upto prog fuel ins' x" by blast
+    from this(1) have "\<exists>ins\<in>instates. steps_upto prog 1 ins ins'" using advance_flat_steps_exact advance_flat_eq by auto
     from this ins' show ?case using steps_upto_suc_bwd by blast
   qed
   thus "x \<in> {st. \<exists>ins\<in>instates. steps_upto prog n ins st}" by blast
@@ -263,7 +263,7 @@ next
       then show ?thesis
       proof(cases "count = 0")
         case True
-        then show ?thesis by (metis "1"(2) Suc.prems(1) continue collect_step_flat_eq collect_step_flat_induct.keep collect_loop_flat.simps(2) steps_exact_zero)
+        then show ?thesis by (metis "1"(2) Suc.prems(1) continue advance_flat_eq advance_flat_induct.keep collect_loop_flat.simps(2) steps_exact_zero)
       next
         case False
         from this 1 have "count = 1" by simp
@@ -273,7 +273,7 @@ next
           case 1 then show ?thesis by simp
         next
           case (2 cmd pc st s n)
-          then show ?thesis using Suc.prems(1) collect_step_flat_eq collect_step_flat_induct.intros(2) continue step_all_flat.intros steps_exact_zero by auto
+          then show ?thesis using Suc.prems(1) advance_flat_eq advance_flat_induct.intros(2) continue step_all_flat.intros steps_exact_zero by auto
         qed
       qed
     qed
@@ -285,6 +285,6 @@ fun errors_all_flat :: "program \<Rightarrow> state set \<Rightarrow> interpret_
 
 fun errors_loop_flat :: "program \<Rightarrow> fuel \<Rightarrow> state set \<Rightarrow> interpret_error set" where
   "errors_loop_flat _ 0 _ = {}" |
-  "errors_loop_flat prog (Suc n) instates = errors_all_flat prog instates \<union> errors_loop_flat prog n (collect_step_flat prog instates)"
+  "errors_loop_flat prog (Suc n) instates = errors_all_flat prog instates \<union> errors_loop_flat prog n (advance_flat prog instates)"
 
 end
